Support for unions (still experimental)

etc/llvm_tests/struct.ll
@@ -3,20 +3,27 @@ target datalayout = "e-m:e-i64:64-f80:128-n8:16:32:64-S128"
 target triple = "x86_64-pc-linux-gnu"
 
 %struct_test = type { i64, i64, i64 }
+%struct_test2 = type { double, double, double }
+%pat_test = type { float, float, double, double }
 
-declare i20000 @llvm.ctlz.i20000(i20000, i1)
+; declare i20000 @llvm.ctlz.i20000(i20000, i1)
+;
+; define i20000 @test(i20000 %x) {
+;   %y = call i20000 @llvm.ctlz.i20000(i20000 %x, i1 true)
+;
+;   ret i20000 %y
+; }
 
-define i20000 @test(i20000 %x) {
-  %y = call i20000 @llvm.ctlz.i20000(i20000 %x, i1 true)
 
-  ret i20000 %y
-}
-
-
-define %struct_test @create_test() {
+define i64 @create_test(%pat_test %arg) {
   start:
 
+    %r1 = alloca %struct_test
+    %r2 = bitcast %struct_test * %r1 to %pat_test *
+    store %pat_test %arg, %pat_test * %r2
+    %r3 = load %struct_test, %struct_test * %r1
 
-    ret %struct_test zeroinitializer
+    %r4 = extractvalue %struct_test %r3, 0
 
+    ret i64 %r4
 }
