etc/llvm_tests/struct_cli.c
@@ -5,44 +5,90 @@
 #include <time.h>
 
 
-typedef struct {
-  int64_t l;
-  int64_t c;
-  int64_t d;
-  //int64_t *data;
-} test;
+typedef union {
+    double f0;
+    struct {
+      char f0;
+      int32_t f1;
+      int32_t f2;
+    }f1;
+  } test ;
 
+
+typedef struct {
+  char a;
+  struct {
+    char b;
+    int64_t c;
+  };
+} test1;
+
+typedef struct {
+  char a;
+  char b;
+  int64_t c;
+} test2;
+
+
+size_t s1 = sizeof(struct{char a;});
+size_t s2 = sizeof(test);
+test t2;
+
+
+typedef union {
+  struct {
+    int32_t a1;
+    int32_t a2;
+    int32_t a3;
+  };
+  struct {
+    int64_t b;
+  };
+} testXX;
 
 test create_test(void);
 
-int64_t read_test(test a) {
-  return a.c;
-}
+// int64_t read_test(test a) {
+//   return a.c;
+// }
 
 
-test create_test2() {
-  test a;
-  a.l=0;
-  a.c=0;
-  a.d=0;
-  return a;
+// test create_test2() {
+//   test a;
+//   a.l=0;
+//   a.c=0;
+//   a.d=0;
+//   return a;
+// }
+
+void foo(testXX *t) {
+  testXX tt;
+
+  tt.a1=-1;
+  tt.b=42;
+
+  *t=tt;
 }
 
 
 int main(int argc, char **argv) {
-  test a;
-  
-  a.l=-1;
-  a.c=-1;
-  a.d=-1;
-//  a.data=(void*)0xFEFEFEFEFEFEFEFE;
+//   test a;
+  testXX aXX;
 
-  printf("%ld,%ld,%ld\n",a.l,a.c,a.d);
-  
-  
-  a = create_test();
+  aXX.a1=-1;
+  aXX.b=42;
 
-  printf("%ld,%ld,%ld\n",a.l,a.c,a.d);
+//   a.l=-1;
+//   a.c=-1;
+//   a.d=-1;
+// //  a.data=(void*)0xFEFEFEFEFEFEFEFE;
+
+//   printf("%ld,%ld,%ld\n",a.l,a.c,a.d);
+  
+  
+//   a = create_test();
+
+//   printf("%ld,%ld,%ld\n",a.l,a.c,a.d);
   
 
   return 0;
