etc/llvm_tests/test_union.ll
@@ -1,0 +1,36 @@
+target datalayout = "e-m:e-i64:64-f80:128-n8:16:32:64-S128"
+target triple = "x86_64-pc-linux-gnu"
+
+%size_t = type i64
+
+%struct1 = type {i32,double}
+%struct2 = type {i64,i64,i64}
+
+
+%structraw = type [
+  (ptrtoint (getelementptr(%struct1*, null, i32 1) to %size_t)) x i8
+]
+
+%structraw = type { [
+  (select(
+    icmp ugt (
+      ptrtoint (getelementptr(%struct1*, null, i32 1) to %size_t),
+      ptrtoint (getelementptr(%struct2*, null, i32 1) to %size_t)
+    ),
+    ptrtoint (getelementptr(%struct1*, null, i32 1) to %size_t),
+    ptrtoint (getelementptr(%struct2*, null, i32 1) to %size_t)
+  )) x i8
+] }
+
+%size_struct1 = ptrtoint (getelementptr(%struct1*, null, i32 1) to %size_t)
+
+
+define i32 main(i32 %argc, i8** %argv) {
+
+
+  ret 0
+}
+
+
+
+
