regression/aggregates/aggr_test_common.h
@@ -1,0 +1,11 @@
+#include <stdio.h>
+#include <stdlib.h>
+#include <stdint.h>
+#include <string.h>
+#include <assert.h>
+
+void error(char const*) __attribute__((noreturn));
+inline void error(char const* msg) {
+  printf("Error: %s\n",msg);
+  exit(1);
+}
