regression/aggregates/dbg_test.c
@@ -1,0 +1,65 @@
+#include "aggr_test_common.h"
+
+typedef union {
+    int16_t f0;
+    struct {
+      double f0;
+    }f1;
+    union {
+      int32_t*f0;
+      float f1;
+      float f2;
+    }f2;
+    double f3;
+    union {
+      float f0;
+    }f4;
+    union {
+      union {
+        int64_t*f0;
+        float f1;
+        float f2;
+        double f3;
+        double f4;
+        struct {
+          int32_t f0;
+          int64_t f1;
+          int16_t f2;
+        }f5;
+        int16_t*f6;
+        int8_t*f7;
+      }f0;
+    }f5;
+    double f6;
+    int16_t f7;
+    int32_t*f8;
+  } testu_t;
+
+
+typedef struct {
+  double f0;
+  testu_t f1;
+  int64_t*f2;
+  double f3;
+  int32_t f4;
+  int16_t*f5;
+}test_t;
+
+typedef struct {
+  int32_t f1; int64_t f2; int16_t f3;
+} testuc_t;
+
+int main() {
+  size_t s1 = sizeof(testuc_t);
+
+  testuc_t* p=0;
+  size_t s2 = (size_t)((void*)(p+1));
+
+  printf("%zd %zd\n",s1,s2);
+
+
+  return 0;
+}
+
+
+
