regression/aggregates/dbg_test.ll
@@ -1,0 +1,56 @@
+; ModuleID = 'dbg_test.c'
+source_filename = "dbg_test.c"
+target datalayout = "e-m:e-p270:32:32-p271:32:32-p272:64:64-i64:64-f80:128-n8:16:32:64-S128"
+target triple = "x86_64-pc-linux-gnu"
+
+%struct.testuc_t = type { i32, i64, i16 }
+
+@.str = private unnamed_addr constant [11 x i8] c"Error: %s\0A\00", align 1
+@.str.1 = private unnamed_addr constant [9 x i8] c"%zd %zd\0A\00", align 1
+
+; Function Attrs: noinline noreturn nounwind optnone uwtable
+define dso_local void @error(i8* %0) #0 {
+  %2 = alloca i8*, align 8
+  store i8* %0, i8** %2, align 8
+  %3 = load i8*, i8** %2, align 8
+  %4 = call i32 (i8*, ...) @printf(i8* getelementptr inbounds ([11 x i8], [11 x i8]* @.str, i64 0, i64 0), i8* %3)
+  call void @exit(i32 1) #4
+  unreachable
+}
+
+declare dso_local i32 @printf(i8*, ...) #1
+
+; Function Attrs: noreturn nounwind
+declare dso_local void @exit(i32) #2
+
+; Function Attrs: noinline nounwind optnone uwtable
+define dso_local i32 @main() #3 {
+  %1 = alloca i32, align 4
+  %2 = alloca i64, align 8
+  %3 = alloca %struct.testuc_t*, align 8
+  %4 = alloca i64, align 8
+  store i32 0, i32* %1, align 4
+  store i64 24, i64* %2, align 8
+  store %struct.testuc_t* null, %struct.testuc_t** %3, align 8
+  %5 = load %struct.testuc_t*, %struct.testuc_t** %3, align 8
+  %6 = getelementptr inbounds %struct.testuc_t, %struct.testuc_t* %5, i64 1
+  %7 = bitcast %struct.testuc_t* %6 to i8*
+  %8 = ptrtoint i8* %7 to i64
+  store i64 %8, i64* %4, align 8
+  %9 = load i64, i64* %2, align 8
+  %10 = load i64, i64* %4, align 8
+  %11 = call i32 (i8*, ...) @printf(i8* getelementptr inbounds ([9 x i8], [9 x i8]* @.str.1, i64 0, i64 0), i64 %9, i64 %10)
+  ret i32 0
+}
+
+attributes #0 = { noinline noreturn nounwind optnone uwtable "correctly-rounded-divide-sqrt-fp-math"="false" "disable-tail-calls"="false" "frame-pointer"="all" "less-precise-fpmad"="false" "min-legal-vector-width"="0" "no-infs-fp-math"="false" "no-jump-tables"="false" "no-nans-fp-math"="false" "no-signed-zeros-fp-math"="false" "no-trapping-math"="false" "stack-protector-buffer-size"="8" "target-cpu"="x86-64" "target-features"="+cx8,+fxsr,+mmx,+sse,+sse2,+x87" "unsafe-fp-math"="false" "use-soft-float"="false" }
+attributes #1 = { "correctly-rounded-divide-sqrt-fp-math"="false" "disable-tail-calls"="false" "frame-pointer"="all" "less-precise-fpmad"="false" "no-infs-fp-math"="false" "no-nans-fp-math"="false" "no-signed-zeros-fp-math"="false" "no-trapping-math"="false" "stack-protector-buffer-size"="8" "target-cpu"="x86-64" "target-features"="+cx8,+fxsr,+mmx,+sse,+sse2,+x87" "unsafe-fp-math"="false" "use-soft-float"="false" }
+attributes #2 = { noreturn nounwind "correctly-rounded-divide-sqrt-fp-math"="false" "disable-tail-calls"="false" "frame-pointer"="all" "less-precise-fpmad"="false" "no-infs-fp-math"="false" "no-nans-fp-math"="false" "no-signed-zeros-fp-math"="false" "no-trapping-math"="false" "stack-protector-buffer-size"="8" "target-cpu"="x86-64" "target-features"="+cx8,+fxsr,+mmx,+sse,+sse2,+x87" "unsafe-fp-math"="false" "use-soft-float"="false" }
+attributes #3 = { noinline nounwind optnone uwtable "correctly-rounded-divide-sqrt-fp-math"="false" "disable-tail-calls"="false" "frame-pointer"="all" "less-precise-fpmad"="false" "min-legal-vector-width"="0" "no-infs-fp-math"="false" "no-jump-tables"="false" "no-nans-fp-math"="false" "no-signed-zeros-fp-math"="false" "no-trapping-math"="false" "stack-protector-buffer-size"="8" "target-cpu"="x86-64" "target-features"="+cx8,+fxsr,+mmx,+sse,+sse2,+x87" "unsafe-fp-math"="false" "use-soft-float"="false" }
+attributes #4 = { noreturn nounwind }
+
+!llvm.module.flags = !{!0}
+!llvm.ident = !{!1}
+
+!0 = !{i32 1, !"wchar_size", i32 4}
+!1 = !{!"clang version 10.0.0-4ubuntu1 "}
