regression/aggregates/Aggregate_Tests.thy
@@ -1,0 +1,302 @@
+theory Aggregate_Tests
+imports "Isabelle_LLVM.LLVM_DS_All"
+begin
+
+  (*
+    Test for aggregates:
+  
+    Main goal:
+      Computations by LLVM, Codegen, and C compiler match on aggregates
+    
+    Coverage goal:
+      * sizeof and alignment computations
+      * include nested aggregates. Anonymous and named. 
+        * play with alignment constraints, e.g. {i8, { i8, i32 } } vs {i8, i8, i32}
+      * include struct and union
+      * include all alignment cases: max-size = max-align, or max-align \<noteq> max-size
+      
+    Test procedure/infrastructure  
+      
+      * generate random aggregate types
+      * convert to LLVM and C types
+      * check Codegen.sizeof T = LLVM.sizeof T
+        * generate LLVM code that compares static sizeof of gep-based sizeof  
+          returns true/false
+      * check Codegen.sizeof T = C.sizeof(T)
+        * generate C program for check
+          reports success/error (message and exit-code)
+      
+      TODO:    
+      * alignment/sizeof check (2)
+        * LLVM code: allocate array of two Ts, write to first, check second is still zeroinitialized
+          returns true/false
+
+      TODO:    
+      * matching check: write struct/union fields in C/LLVM, check in LLVM/C
+                  
+    Overall infrastructure:
+      * command to generate tests: parse type T, write agg_test_T.{ll,c}
+
+      
+  *)
+
+  ML \<open>
+    structure Aggregate_Tests = struct
+      local 
+        open Parser_Util 
+        open LLC_Intermediate
+              
+      in
+      
+        val parse_id = Parse.short_ident
+
+        fun assert_positive n = if n>0 then n else raise Fail("Positive number expected: " ^ quote (Int.toString n))
+                
+        val scan_int_type = unprefix "i" #> Value.parse_nat #> assert_positive #> TInt 
+        
+        val parse_int_type = ident_with (can scan_int_type) >> scan_int_type
+        
+        val is_ptr = String.explode #> forall (fn x => x = #"*")
+        
+        val parse_ptr = kind_with Token.Sym_Ident is_ptr
+        
+        fun parse_type_np s = (
+             parse_int_type
+          || pkw "float" >> K TFloat
+          || pkw "double" >> K TDouble
+          || parse_id >> TNamed
+          || pcm "{" |-- Parse.enum1 "," parse_type --| pcm "}" >> TStruct
+          || pcm "u{" |-- Parse.enum1 "," parse_type --| pcm "}" >> TUnion
+        ) s
+        and parse_type s = (
+          parse_type_np -- (Scan.repeat parse_ptr >> map String.explode >> flat) >> (fn (T,ms) => fold (K TPtr) ms T)
+        ) s
+        
+    
+        val kws = ["float","double","{","}","u{",","]
+    
+        val check_type = parse_inner kws parse_type
+  
+      end
+  
+      
+      local open C_Interface in
+      
+        infix 3 >>=
+      
+        fun m >>= f = map f m |> flat
+        
+        fun mapM _ [] = single []
+          | mapM f (x::xs) = f x >>= (fn x' => mapM f xs >>= (fn xs' => single (x'::xs')))
+        
+        
+        fun cty_names _ (CTYO_PRIM p) = CTY_PRIM p
+          | cty_names pre (CTYO_PTR t) = CTY_PTR (cty_names pre t)
+          | cty_names _ (CTYO_NAMED s) = CTY_NAMED s
+          | cty_names pre (CTYO_STRUCT flds) = CTY_STRUCT (map (cty_names_fld pre) (tag_list 0 flds))
+          | cty_names pre (CTYO_UNION flds) = CTY_UNION (map (cty_names_fld pre) (tag_list 0 flds))
+        and 
+            cty_names_fld pre (i,FLDO_NAMED (SOME t,_)) = FLD_NAMED (cty_names pre t, "f"^pre^Int.toString i)
+          | cty_names_fld _ _ = error "cty_names_fld: no type-info for field"
+      
+        (*  
+        fun cty_names _ (CTYO_PRIM p) = single (CTY_PRIM p)
+          | cty_names pre (CTYO_PTR t) = map CTY_PTR (cty_names pre t)
+          | cty_names _ (CTYO_NAMED s) = single (CTY_NAMED s)
+          | cty_names pre (CTYO_STRUCT flds) = map CTY_STRUCT (mapM (cty_names_fld pre) (tag_list 0 flds))
+          | cty_names pre (CTYO_UNION flds) = map CTY_UNION (mapM (cty_names_fld pre) (tag_list 0 flds))
+        and 
+            cty_names_fld pre (i,FLDO_NAMED (SOME (t as CTYO_STRUCT flds),_)) = 
+              (cty_names pre t >>= (fn t => single (FLD_NAMED (t, "f"^pre^Int.toString i))))
+            @ map FLD_ANON (mapM (cty_names_fld (pre^"n")) (tag_list 0 flds))
+            
+          | cty_names_fld pre (i,FLDO_NAMED (SOME t,_)) = cty_names pre t >>= (fn t => single (FLD_NAMED (t, "f"^pre^Int.toString i)))
+          | cty_names_fld _ _ = error "cty_names_fld: no type-info for field"
+        *)
+      
+      
+      end
+      
+      local open LLVM_Builder in
+      
+        fun mk_ll_sizeof_test b name lty = let
+          val _ = open_proc b (SOME (mkty_i 8)) name [] []
+          val dy_sz = mk_size_of b (SOME "") lty
+          val st_sz = sizeof_ty b lty |> mkc_i (size_t b)
+          val res = mk_icmp_instr "eq" b (SOME "") dy_sz st_sz
+          val res = mk_conv_instr "zext" b (SOME "") res (mkty_i 8)
+          val _ = mk_return b (SOME res)
+          val _ = close_proc b
+        in
+          ()
+        end
+
+        fun mk_ll_sizeof_get b name lty = let
+          val _ = open_proc b (SOME (size_t b)) name [] []
+          val st_sz = sizeof_ty b lty |> mkc_i (size_t b)
+          val _ = mk_return b (SOME st_sz)
+          val _ = close_proc b
+        in
+          ()
+        end
+              
+      end
+      
+      local
+        open Simple_PP 
+      in      
+      
+      
+      end
+  
+      fun make_test ctxt i llT = let
+        val cT = C_Interface.cty_of_lty llT |> cty_names "" |> C_Interface.ctype_to_Cs
+    
+        val name = "aggr_test_" ^ Int.toString (i)
+        val name_get = name ^ "_get"
+        val name_test = name ^ "_test"
+    
+        val using_master_directory =
+          File.full_path (Resources.master_directory (Proof_Context.theory_of ctxt));
+        
+        val base_path = ("../../regression/aggregates/generated/" ^ name)
+          |> Path.explode |> using_master_directory
+        val ll_path = Path.ext "gen.ll" base_path
+        val c_path = Path.ext "c" base_path
+          
+        val b = LLVM_Builder.builder LLVM_Builder.target_x86_64_linux
+            
+        val lty = LLC_Backend.llc_ty b llT
+        val sz = LLVM_Builder.sizeof_ty b lty
+        val _ = mk_ll_sizeof_get b name_get lty
+        val _ = mk_ll_sizeof_test b name_test lty
+        
+        (*val _ = @{print} ll_path*)
+        val _ = LLVM_Builder.string_of b |> File.write ll_path
+        
+        
+        local open C_Interface Simple_PP in
+          val decls = fbrks [
+            block [word "char",fsep,word name_test,nword "()",nword ";"],
+            block [word "size_t",fsep,word name_get,nword "()",nword ";"],
+            fbrk,
+            block [word "typedef",cT,word "test_t",nword ";"],
+            fbrk,
+            block [word "test_t",word "test_v",nword ";"],
+            block [word "size_t",word "test_size",nword "=",word "sizeof(test_t)",nword ";"]
+          ] 
+          
+          val C_test = block [
+            line [nword "if (sizeof(test_t) != ", int sz, nword ") error(\"static vs C size test failed\");"]
+          ]
+    
+          val C_tests = fbrks [
+            line [nword "if (!",word name_test,nword "()) error(\"static vs dynamic LLVM size test failed\");"],
+            C_test]
+          
+          val ccode = fbrks [
+            word "#include \"../aggr_test_common.h\"",
+            decls,
+            word "int main() {",
+            block_indent 1 [C_tests,word "return 0;",fbrk],
+            word "}"
+          ]
+          
+        end  
+        
+        val _ = ccode |> Simple_PP.string_of |> File.write c_path
+      in () end    
+            
+    end
+  \<close>
+  
+  
+  
+  ML \<open>
+    (*  Adapted from Larry's Random.ML, to allow for control over seeds *)
+    signature RANDOM_GEN =
+    sig
+      type T
+      val make: real -> T
+      val random: T -> real
+      val random_range: T -> int -> int -> int
+      exception RANDOM_GEN;
+    end;
+    
+    structure Random_Gen: RANDOM_GEN =
+    struct
+    
+      fun rmod x y = x - y * Real.realFloor (x / y);
+  
+      type T = real Synchronized.var
+      
+      fun make seed = Synchronized.var "Rand_Gen seed" seed
+        
+      local
+        val a = 16807.0;
+        val m = 2147483647.0;
+      in
+      
+        fun random rgstate =
+          Synchronized.change_result rgstate
+            (fn r => let val r' = rmod (a * r) m in (r', r') end);
+      
+      end;
+    
+      exception RANDOM_GEN;
+    
+      fun random_range rgstate l h =
+        if h < l orelse l < 0 then raise RANDOM_GEN
+        else l + Real.floor (rmod (random rgstate) (real (h - l + 1)));
+      
+    end;
+  \<close>
+  
+  
+  ML \<open>
+    fun random_el rg xs = nth xs (Random_Gen.random_range rg 0 (length xs - 1))
+    
+    fun random_wel rg xs = map (uncurry replicate) xs |> flat |> random_el rg  (* TODO: Inefficient *)
+    
+
+    local    
+      open LLC_Intermediate
+    in
+      fun llc_random_int rg = TInt (random_el rg [8,16,32,64])
+    
+      fun llc_random_prim rg = random_el rg [llc_random_int, K TFloat, K TDouble] rg
+    
+      fun llc_random_field_num rg = random_wel rg (
+          map (pair 8) (1 upto 2)
+        @ map (pair 4) (3 upto 4)
+        @ map (pair 2) (5 upto 8)
+        @ map (pair 1) (9 upto 16)
+      )
+      
+      
+      fun max a b = if a>=b then a else b
+      
+      fun llc_random_ty d rg = random_wel rg [(8,llc_random_prim),(2,llc_random_ptr),(max 1 (4-d),llc_random_struct (d+1)),(max 1 (4-d),llc_random_union (d+1))] rg
+      and llc_random_ptr rg = TPtr (llc_random_int rg)
+      and llc_random_fields d rg = map (llc_random_ty d) (replicate (llc_random_field_num rg) rg)
+      and llc_random_struct d rg = TStruct (llc_random_fields d rg)
+      and llc_random_union d rg = TUnion (llc_random_fields d rg)
+      
+    
+    end    
+    
+    val rg = Random_Gen.make 1.0
+    
+    val tests = map (llc_random_struct 0) (replicate 1000 rg) |> distinct (op =) |> tag_list 1
+
+    (*val tests = let open LLC_Intermediate in [(1,TUnion [TDouble, TStruct [TInt 8, TInt 32, TInt 32]])] end*)
+    
+    val _ = writeln ("Creating " ^ Int.toString (length tests) ^ " tests")
+    
+    
+    val _ = map (uncurry (Aggregate_Tests.make_test @{context})) tests
+    val _ = writeln ("Done")
+  \<close>
+
+
+end
