regression/aggregates/testall.sh
@@ -1,0 +1,53 @@
+#!/bin/bash
+
+set -e
+
+echo "Aggregate Tests"
+
+echo "  Cleaning up"
+
+rm -f generated/*
+
+echo "  Building thy and generating tests"
+
+isabelle build -c -d . Aggregate_Tests
+
+
+exitcode=0
+
+function error() {
+  echo $1
+  exitcode=1
+}
+
+echo "  Compiling and running generated tests"
+
+ntest=0
+
+for C_FILE in generated/aggr_test_*.c; do
+
+  STEM="${C_FILE%.c}"
+
+  LL_FILE="$STEM.gen.ll"
+  BIN_FILE="$STEM"
+
+  if clang $C_FILE $LL_FILE -o $BIN_FILE; then
+    if ! ./$BIN_FILE; then
+      clang -S -emit-llvm $C_FILE
+      error "FAILED TEST: $STEM"
+    fi
+  else
+    error "FAILED COMPILATION: $STEM"
+  fi
+
+  ntest=$((ntest+1))
+done
+
+if test $exitcode -eq 0; then
+  echo "DONE (Aggregate Tests) $ntest tests completed"
+else
+  echo "ERROR (Aggregate Tests)"
+fi  
+
+exit $exitcode
+
